clightplus/mem/ClightPlusMemAux.v
@@ -103,14 +103,14 @@ Proof.
   - hexploit IHSTORE_ZEROS; et. i. des. eapply H0. nia.
 Qed.
 
-Lemma match_mem_getN f (c d: Maps.ZMap.t memval) n p
+(* Lemma match_mem_getN f (c d: Maps.ZMap.t memval) n p
     (MM: forall i mv, Maps.ZMap.get i c = mv -> Maps.ZMap.get i d = f mv)
   :
     Mem.getN n p d = map f (Mem.getN n p c).
 Proof.
   revert p. induction n; i; ss.
   rewrite IHn. f_equal. erewrite <- MM; try reflexivity.
-Qed.
+Qed. *)
 
 Lemma proj_determines_decode_val l :
   proj_bytes l = None -> proj_fragment l = None -> decode_val Mptr l = Vundef.
